\subsection{Cost functions}

\subsubsection{Multi-class classification}

\begin{frame}\frametitle{Data representation}
	\textbf{Prediction of class labels}\\[4mm]
	observations: $\Big\{ \Big( \vec{x}^{(\alpha)}, y_T^{(\alpha)} 
		\Big) \Big\}, \quad \alpha \in  \{1, \ldots, p\}$\\
			$c$ classes $C_k, \quad k \in \{1, \ldots, c\}
		\quad\Rightarrow\quad y_T^{(\alpha)} \in \{1, \ldots, k\}$
	\vspace{8mm}
	\pause
	
	\textbf{Prediction of class probabilities}\\
	\begin{block}{1-out-of-c code}
		\begin{equation*}
			y_{Tk}^{(\alpha)} = \left 
			\{ \begin{array}{lll}
			0, & \vec{x}^{(\alpha)} \notin C_k  \\
			1, & \vec{x}^{(\alpha)} \in C_k
			\end{array} \right.
			\quad \Rightarrow 
			\text{binary vector $\vec y_T^{(\alpha)}$, one non-zero element}
		\end{equation*}
		Limiting case of probabilities: true labels are known.
	\end{block}
\end{frame}


% -----------------------------------------------------------------------------
\begin{frame}\frametitle{Model class}
	\[ \begin{array}{ll}
		\begin{array}{l}
			%\includegraphics[height=4cm]{img/section1_fig37}
		\end{array}
		&
		\begin{array}{l}
			\text{Probabilistic interpretation} \\
			\text{of network output:}\\[1mm]
			y_{k (\vec{x};\vec{w})} \coloneqq P(\vec{x} \in C_k; \vec{w}) \\[2mm]
			\begin{array}{lcl}
				0 \leq & y_{k (\vec{x};\vec{w})} & \leq 1 \\[1mm]
					   & \sum\limits_{k=1}^c 
					   		y_{k (\vec{x};\vec{w})} & = 1
			\end{array}
		\end{array}
	\end{array} \]
\end{frame}

\begin{frame}\frametitle{Optimization via gradient descent (on-line)}
From minimizing KL-divergence to multi-class cross entropy:
	\begin{equation}
			\frac{\partial e}{\partial \vec{w}}
		=  - \frac{\partial}{\partial \vec{w}} 
		  	\sum_{k = 1}^c y_{Tk} 
		  	\ln \big(y_{k (\vec{x}; \vec{w})}\big)
	\end{equation}
	with
	\begin{equation}
		  	y_{k (\vec{x};\vec{w})} = \frac{\exp h_{k (\vec{x};\vec{w})}}
		  		{\sum_l \exp h_{l (\vec{x};\vec{w})}}
	\end{equation}
	due to softmax normalization.
	For brevity:
	\begin{equation}
		  	y_{k (\vec{x};\vec{w})} = 
		  	y_{k} = \frac{\exp h_{k}}
		  		{\sum_l \exp h_{l}}
	\end{equation}
	\notesonly{
	(don't forget that $y_k$, $h_k$ and $h_l$ are all functions of $\vec w$)
	}
	\begin{align}
	\frac{\partial e}{\partial \vec{w}} =
	\frac{\partial}{\partial \vec{w}} 
		  	\sum_{k = 1}^c y_{Tk}
		  	\ln \big(y_{k}\big)
		& \stackrel{\substack{\text{chain}\\\text{rule}}}{=} 
		\sum\limits_{k = 1}^c y_{Tk} \cdot \frac{1}{y_k} \cdot \frac{\partial y_k}{\partial \vec{w}}
	\end{align}
	Compute $\frac{\partial y_k}{\partial \vec{w}}$ (i.e. derivative of softmax normalization):
	

\end{frame}

\begin{frame}\frametitle{Derivative of softmax normalization}
\only<1>{
	\begin{align}
		\frac{\partial y_k}{\partial \vec{w}}
		& = \frac{\partial}{\partial \vec{w}}
		\left( 
		\frac{\exp h_{k}}
		{\sum_l \exp h_{l}}
		\right)
		 = \frac{\partial}{\partial \vec{w}} 
		 \left( 
		\frac{u}{v}
		  \right)
	\end{align}
	
	where
	\begin{align}
	u := \exp h_{k} \quad &\leadsto \quad u' := \exp h_{k} \frac{\partial h_k}{\partial \vec{w}}\\
	v := \sum_l \exp h_{l} \quad &\leadsto \quad v' := \sum_l \left( \exp h_{l} \frac{\partial h_l}{\partial \vec{w}} \right)
	\end{align}
	
	Using the quotient rule:
	}
	\begin{align}
	\only<1>{
	\frac{\partial y_k}{\partial \vec{w}}
	&= 
		\frac{u'v - v'u}
		{v^2}
	=
		\frac{u'v}
		{v^2}
		-
		\frac{v'u}
		{v^2}\\
	&=  \frac{\exp h_{k} \cdot \frac{\partial h_k}{\partial \vec{w}} \cdot \sum_l \exp h_{l}}{ \left(\sum_l \exp h_{l} \right)^2 }
	-
	\frac{\exp h_{k} \sum_l \left( \exp h_{l} \cdot \frac{\partial h_l}{\partial \vec{w}} \right) }{ \left(\sum_l \exp h_{l} \right)^2 }\\
	}
	\only<2->{
	\slidesonly{\frac{\partial y_k}{\partial \vec{w}}}
	&=  \frac{\exp h_{k} \cdot \frac{\partial h_k}{\partial \vec{w}} \cdot \cancel{\sum_l \exp h_{l}}}{ \left(\sum_l \exp h_{l} \right)^{\cancel{2}} }
	-
	\frac{\exp h_{k} \sum_l \left( \exp h_{l} \cdot \frac{\partial h_l}{\partial \vec{w}} \right) \cdot }{ \left(\sum_l \exp h_{l} \right)^2 }\\
	}
	\only<3->{
	&=  \;\; \frac{\exp h_{k}}{ \sum_l \exp h_{l} } \cdot \frac{\partial h_k}{\partial \vec{w}} \;\;
	- \;\;
	\frac{\exp h_{k}}{ \sum_l \exp h_{l}  } \cdot 
	\frac{\sum_l \left( \exp h_{l} \cdot \frac{\partial h_l}{\partial \vec{w}} \right) }{ \sum_l \exp h_{l} }\\
	}
	\only<4->{
	&=  \qquad y_k \cdot \frac{\partial h_k}{\partial \vec{w}} \;\;
	- \;\;
	y_k \cdot 
	\frac{\sum_l \left( \exp h_{l} \cdot \frac{\partial h_l}{\partial \vec{w}} \right) }{ \sum_l \exp h_{l} }\\
	}
	\only<5->{
	&=  \qquad y_k \cdot \frac{\partial h_k}{\partial \vec{w}} \;\;
	- \;\;
	y_k \cdot 
	\sum_l \left(\frac{ \exp h_{l}  }{ \sum_l \exp h_{l} } \right) \cdot \frac{\partial h_l}{\partial \vec{w}} \\
	}
	\only<6->{
	&=  \qquad y_k \cdot \frac{\partial h_k}{\partial \vec{w}} \;\;
	- \;\;
	y_k \cdot 
	\sum_l y_{l} \cdot \frac{\partial h_l}{\partial \vec{w}}
	}
	\end{align}

\end{frame}
\begin{frame}
	Plugging this back into our expression for $\partial e/\partial \vec w$:
	\begin{align}
		\frac{\partial e}{\partial \vec{w}} 
		&= -
		\sum\limits_{k = 1}^c y_{Tk} \cdot \frac{1}{y_k} \cdot \frac{\partial y_k}{\partial \vec{w}}\\
		&= -\sum\limits_{k = 1}^c  \frac{y_{Tk}}{\cancel{y_k}} \cdot \left( \cancel{y_k} \cdot \frac{\partial h_k}{\partial \vec{w}} 
		- 
		\cancel{y_k} \cdot 
		\sum_l y_{l} \cdot \frac{\partial h_l}{\partial \vec{w}} \right)\\
	\only<2->{
		&= -\sum\limits_{k = 1}^c  {y_{Tk}} \cdot \frac{\partial h_k}{\partial \vec{w}} 
		+ \underbrace{\left(\sum\limits_{k = 1}^c  {y_{Tk}}\right)}_{\only<2>{=?}\only<3->{=1}} \cdot
		\sum_l y_{l} \cdot \frac{\partial h_l}{\partial \vec{w}}\\
		}
	\only<4->{
		&= -\sum\limits_{k = 1}^c  {y_{Tk}} \cdot \frac{\partial h_k}{\partial \vec{w}} 
		+ 
		\sum_{l=1}^c y_{l} \cdot \frac{\partial h_l}{\partial \vec{w}}\\
		}
	\only<5->{
		&= {\color{red}-}\sum\limits_{k = 1}^c  {y_{Tk}} \cdot \frac{\partial h_k}{\partial \vec{w}} 
		{\color{red}+} 
		\sum\limits_{k = 1}^c y_{k} \cdot \frac{\partial h_k}{\partial \vec{w}}\\
		&= \sum\limits_{k = 1}^c  \left( y_{k}
		{\color{red}-} y_{Tk}
		 \right) \cdot \frac{\partial h_k}{\partial \vec{w}}
		 }
	\end{align}
\end{frame}
\begin{frame}
	Since we evaluate the error for each individual pair $(\vec x^{(\alpha)}, \vec y_T^{(\alpha)})$:
	\begin{align}
	\frac{\partial e^{(\alpha)}}{\partial \vec{w}}
		& =  \sum\limits_{k = 1}^c \Big( y_{k (\vec{x}^{(\alpha)}; 
			\vec{w})} - y_{Tk}^{(\alpha)} \Big) 
				\underbrace{\frac{\partial h_{k (\vec{x}^{(\alpha)}; 
				              \vec{w})}}{\partial \vec{w}}}_{
				          \substack{\text{via}\\ \text{backprop}}}
	\end{align}
	
\end{frame}

